src/compiler/meta/OCL_compiler_parser_META.thy
@@ -102,6 +102,7 @@ definition "i_of_floor a b = rec_floor
   (b \<open>Floor3\<close>)"
 
 definition "i_of_ocl_deep_embed_ast a b = rec_ocl_deep_embed_ast
+  (ap1 a (b \<open>OclAstEnum\<close>) (i_of_ocl_enum a b))
   (ap2 a (b \<open>OclAstClassRaw\<close>) (i_of_floor a b) (i_of_ocl_class_raw a b (K i_of_unit)))
   (ap1 a (b \<open>OclAstAssociation\<close>) (i_of_ocl_association a b (K i_of_unit)))
   (ap2 a (b \<open>OclAstAssClass\<close>) (i_of_floor a b) (i_of_ocl_ass_class a b))
